Attempt2/Compose.dfy
@@ -1,0 +1,99 @@
+module Compose {
+
+  import opened Circ
+  import opened Eval
+  import opened Utils
+  import opened MapFunction
+
+  ghost opaque predicate ComposedValid(c: Circuit, e1: Equiv, e2: Equiv) {
+    CircuitValid(c) &&
+    EquivValid(c, e1) &&
+    EquivValid(c, e2) &&
+    EquivTrue(c, e1) &&
+    EquivTrue(c, e2) &&
+    SetsNoIntersection(e1.sc, e2.sc) &&
+    ScValid(c, e1.sc) && // unnecessary but EquivValid is opaque
+    ScValid(c, e2.sc) && // unnecessary but EquivValid is opaque
+    (NPBetweenSubcircuits(c, e1.sc, e2.sc) == {})
+  }
+
+  lemma SetsNoIntersectionFromComposedValid(c: Circuit, e1: Equiv, e2: Equiv)
+  requires ComposedValid(c, e1, e2)
+  ensures SetsNoIntersection(e1.sc, e2.sc)
+  {
+    reveal ComposedValid();
+  }
+
+  lemma CircuitValidFromComposedValid(c: Circuit, e1: Equiv, e2: Equiv)
+  requires ComposedValid(c, e1, e2)
+  ensures CircuitValid(c)
+  {
+    reveal ComposedValid();
+  }
+
+
+  function {:vcs_split_on_every_assert} ComposeEquiv(c: Circuit, e1: Equiv, e2: Equiv): (r: Equiv)
+    requires ComposedValid(c, e1, e2)
+    ensures EquivValid(c, r)
+  {
+    reveal ComposedValid();
+    reveal EquivValid();
+    var combined_input_keys := ComposeEquivInputs(c, e1, e2);
+    var e := Equiv(
+      CombineSets(e1.sc, e2.sc),
+      combined_input_keys,
+      e1.outputs + e2.outputs,
+      (combined_inputs: map<NP, bool>) requires combined_inputs.Keys == combined_input_keys => ComposeEquivF(c, e1, e2, combined_inputs)
+    );
+    e
+  }
+
+  function ComposeEquivInputs(c: Circuit, e1: Equiv, e2: Equiv): (r: set<NP>)
+    requires ComposedValid(c, e1, e2)
+    ensures forall np :: np in e1.inputs ==> np in r
+  {
+    reveal ComposedValid();
+    reveal EquivValid();
+    (set np | np in (e1.inputs + e2.inputs) && np !in NPBetweenSubcircuits(c, e2.sc, e1.sc))
+  }
+
+  lemma ComposeEquivInputsCorrect(c: Circuit, e1: Equiv, e2: Equiv)
+    requires ComposedValid(c, e1, e2)
+    ensures ScValid(c, e1.sc + e2.sc)
+    ensures
+      ScInputBoundary(c, e1.sc + e2.sc) == ComposeEquivInputs(c, e1, e2)
+  {
+    reveal ComposedValid();
+    reveal EquivValid();
+  }
+
+  function CalculateE2Inputs(c: Circuit, e1: Equiv, e2: Equiv, knowns: map<NP, bool>): (r: map<NP, bool>)
+    requires ComposedValid(c, e1, e2)
+    requires knowns.Keys == ComposeEquivInputs(c, e1, e2)
+  {
+    reveal ComposedValid();
+    reveal EquivValid();
+    var mf1 := MapFunction(e1.inputs, e1.outputs, e1.f);
+    var mf2 := MapFunction(e2.inputs, e2.outputs, e2.f);
+    assert MapFunctionValid(mf1);
+    assert MapFunctionValid(mf2);
+    var e2_inputs_from_e1_keys := NPBetweenSubcircuits(c, e2.sc, e1.sc);
+    var e2_inputs_from_e1 := (map np | np in e2_inputs_from_e1_keys :: np := c.PortSource[np]);
+    GetInputs2(mf1, mf2, e2_inputs_from_e1, knowns)
+  }
+
+  function ComposeEquivF(c: Circuit, e1: Equiv, e2: Equiv, combined_inputs: map<NP, bool>): (r: map<NP, bool>)
+    requires ComposedValid(c, e1, e2)
+    requires combined_inputs.Keys == ComposeEquivInputs(c, e1, e2)
+  {
+    reveal ComposedValid();
+    reveal EquivValid();
+    var mf1 := MapFunction(e1.inputs, e1.outputs, e1.f);
+    var mf2 := MapFunction(e2.inputs, e2.outputs, e2.f);
+    assert MapFunctionValid(mf1);
+    assert MapFunctionValid(mf2);
+    var e2_inputs_from_e1_keys := NPBetweenSubcircuits(c, e2.sc, e1.sc);
+    var e2_inputs_from_e1 := (map np | np in e2_inputs_from_e1_keys :: np := c.PortSource[np]);
+    ComposeMapFunction(mf1, mf2, e2_inputs_from_e1, combined_inputs)
+  }
+}
