Attempt2/ComposeEval.dfy
@@ -1,0 +1,504 @@
+module ComposeEval {
+
+  import Std.Collections.Seq
+
+  import opened Circ
+  import opened Eval
+  import opened Compose
+  import opened Utils
+  import opened MapFunction
+
+  lemma NPNotInPathHelper(np: NP, sc1: set<CNode>, sc2: set<CNode>, prepath: seq<NP>, path: seq<NP>)
+    requires np.n in sc1
+    requires SetsNoIntersection(sc1, sc2)
+    requires forall np :: np in prepath ==> np.n in sc2
+    requires forall np :: np in path ==> np.n in sc1
+    ensures (np in path) == (np in (prepath + path))
+  {
+  }
+  
+  lemma {:vcs_split_on_every_assert} EvaluateONPBinaryComposed1(
+      c: Circuit, e1: Equiv, e2: Equiv, prepath: seq<NP>, path: seq<NP>, knowns: map<NP, bool>)
+    requires CircuitValid(c)
+    requires ComposedValid(c, e1, e2)
+    requires knowns.Keys == ComposeEquivInputs(c, e1, e2)
+    requires forall np :: np in prepath ==> np.n in e2.sc
+    requires forall np :: np in path ==> np.n in e1.sc
+    requires EvaluateONPBinaryRequirements(c, path, knowns)
+    requires EvaluateONPBinaryRequirements(c, prepath + path, knowns)
+    ensures
+      var knowns_1 := ExtractMap(knowns, e1.inputs);
+      var np := Seq.Last(path);
+      (EvaluateONPBinary(c, path, knowns) == EvaluateONPBinary(c, path, knowns_1)) &&
+      (Simpl(EvaluateONPBinary(c, path, knowns)) == Simpl(EvaluateONPBinary(c, prepath+path, knowns)))
+    decreases |NodesNotInPath(c, prepath + path)|, 3
+  {
+    var knowns_1 := ExtractMap(knowns, e1.inputs);
+    var head := Seq.Last(path);
+    assert NodeValid(c, head.n);
+    var inp_0 := NP(head.n, INPUT_0);
+    var inp_1 := NP(head.n, INPUT_1);
+    SetsNoIntersectionFromComposedValid(c, e1, e2);
+    NPNotInPathHelper(inp_0, e1.sc, e2.sc, prepath, path);
+    NPNotInPathHelper(inp_1, e1.sc, e2.sc, prepath, path);
+    if inp_0 in path {
+      assert (EvaluateONPBinary(c, path, knowns) == EvaluateONPBinary(c, path, knowns_1));
+      assert (Simpl(EvaluateONPBinary(c, path, knowns)) == Simpl(EvaluateONPBinary(c, prepath+path, knowns)));
+    } else if inp_1 in path {
+      assert (EvaluateONPBinary(c, path, knowns) == EvaluateONPBinary(c, path, knowns_1));
+      assert (Simpl(EvaluateONPBinary(c, path, knowns)) == Simpl(EvaluateONPBinary(c, prepath+path, knowns)));
+    } else {
+      NodesNotInPathDecreases(c, prepath + path, inp_0);
+      NodesNotInPathDecreases(c, prepath + path, inp_1);
+      StillHasNoDuplicates(path, inp_0);
+      StillHasNoDuplicates(prepath + path, inp_0);
+      assert (prepath + path) + [inp_0] == prepath + (path + [inp_0]);
+      assert Seq.HasNoDuplicates(prepath + (path + [inp_0]));
+      StillHasNoDuplicates(path, inp_1);
+      StillHasNoDuplicates(prepath + path, inp_1);
+      assert (prepath + path) + [inp_1] == prepath + (path + [inp_1]);
+      assert Seq.HasNoDuplicates(prepath + (path + [inp_1]));
+      EvaluateINPInnerComposed1(c, e1, e2, prepath, path + [inp_0], knowns);
+      EvaluateINPInnerComposed1(c, e1, e2, prepath, path + [inp_1], knowns);
+      assert (EvaluateONPBinary(c, path, knowns) == EvaluateONPBinary(c, path, knowns_1));
+      assert (Simpl(EvaluateONPBinary(c, path, knowns)) == Simpl(EvaluateONPBinary(c, prepath+path, knowns)));
+    }
+  }
+
+  lemma {:vcs_split_on_every_assert} EvaluateONPBinaryComposed2(
+      c: Circuit, e1: Equiv, e2: Equiv, path: seq<NP>, knowns: map<NP, bool>)
+    requires CircuitValid(c)
+    requires ComposedValid(c, e1, e2)
+    requires knowns.Keys == ComposeEquivInputs(c, e1, e2)
+    requires forall np :: np in path ==> np.n in e2.sc
+    requires EvaluateONPBinaryRequirements(c, path, knowns)
+    ensures
+      var knowns_2 := CalculateE2Inputs(c, e1, e2, knowns);
+      var np := Seq.Last(path);
+      (EvaluateONPBinary(c, path, knowns) == EvaluateONPBinary(c, path, knowns_2))
+    decreases |NodesNotInPath(c, path)|, 3
+  {
+    var nk := c.NodeKind[path[|path|-1].n];
+    var head := path[|path|-1];
+    assert NodeValid(c, head.n);
+    var inp_0 := NP(head.n, INPUT_0);
+    var inp_1 := NP(head.n, INPUT_1);
+    if inp_0 in path {
+    } else if inp_1 in path {
+    } else {
+      NodesNotInPathDecreases(c, path, inp_0);
+      NodesNotInPathDecreases(c, path, inp_1);
+      StillHasNoDuplicates(path, inp_0);
+      StillHasNoDuplicates(path, inp_1);
+      EvaluateINPInnerComposed2(c, e1, e2, path + [inp_0], knowns);
+      EvaluateINPInnerComposed2(c, e1, e2, path + [inp_1], knowns);
+    }
+  }
+
+  lemma {:vcs_split_on_every_assert} EvaluateONPUnaryComposed1(
+      c: Circuit, e1: Equiv, e2: Equiv, prepath: seq<NP>, path: seq<NP>, knowns: map<NP, bool>)
+    requires CircuitValid(c)
+    requires ComposedValid(c, e1, e2)
+    requires knowns.Keys == ComposeEquivInputs(c, e1, e2)
+    requires forall np :: np in prepath ==> np.n in e2.sc
+    requires forall np :: np in path ==> np.n in e1.sc
+    requires EvaluateONPUnaryRequirements(c, path, knowns)
+    requires EvaluateONPUnaryRequirements(c, prepath+path, knowns)
+    ensures
+      var knowns_1 := ExtractMap(knowns, e1.inputs);
+      var np := Seq.Last(path);
+      (EvaluateONPUnary(c, path, knowns) == EvaluateONPUnary(c, path, knowns_1)) &&
+      (Simpl(EvaluateONPUnary(c, path, knowns)) == Simpl(EvaluateONPUnary(c, prepath+path, knowns)))
+    decreases |NodesNotInPath(c, prepath + path)|, 3
+  {
+    var head := path[|path|-1];
+    var inp_0 := NP(head.n, INPUT_0);
+    SetsNoIntersectionFromComposedValid(c, e1, e2);
+    NPNotInPathHelper(inp_0, e1.sc, e2.sc, prepath, path);
+    if inp_0 in path {
+    } else {
+      NodesNotInPathDecreases(c, prepath + path, inp_0);
+      StillHasNoDuplicates(path, inp_0);
+      StillHasNoDuplicates(prepath + path, inp_0);
+      assert (prepath + path) + [inp_0] == prepath + (path + [inp_0]);
+      assert Seq.HasNoDuplicates(prepath + (path + [inp_0]));
+      EvaluateINPInnerComposed1(c, e1, e2, prepath, path + [inp_0], knowns);
+    }
+  }
+
+  lemma {:vcs_split_on_every_assert} EvaluateONPUnaryComposed2(
+      c: Circuit, e1: Equiv, e2: Equiv, path: seq<NP>, knowns: map<NP, bool>)
+    requires CircuitValid(c)
+    requires ComposedValid(c, e1, e2)
+    requires knowns.Keys == ComposeEquivInputs(c, e1, e2)
+    requires forall np :: np in path ==> np.n in e2.sc
+    requires EvaluateONPUnaryRequirements(c, path, knowns)
+    ensures
+      var knowns_2 := CalculateE2Inputs(c, e1, e2, knowns);
+      var np := Seq.Last(path);
+      EvaluateONPUnary(c, path, knowns) == EvaluateONPUnary(c, path, knowns_2)
+    decreases |NodesNotInPath(c, path)|, 3
+  {
+    var head := path[|path|-1];
+    var inp_0 := NP(head.n, INPUT_0);
+    if inp_0 in path {
+    } else {
+      NodesNotInPathDecreases(c, path, inp_0);
+      StillHasNoDuplicates(path, inp_0);
+      EvaluateINPInnerComposed2(c, e1, e2, path + [inp_0], knowns);
+    }
+  }
+
+  lemma HasNoDuplicatesMeansHeadNotInTail<T>(a: seq<T>)
+    requires |a| > 0
+    requires Seq.HasNoDuplicates(a)
+    ensures
+      var head := Seq.Last(a);
+      var tail := Seq.DropLast(a);
+      head !in tail
+  {
+    reveal Seq.HasNoDuplicates();
+  }
+
+  lemma {:vcs_split_on_every_assert} EvaluateINPInnerComposed1(c: Circuit, e1: Equiv, e2: Equiv, prepath: seq<NP>, path: seq<NP>, knowns: map<NP, bool>)
+    requires CircuitValid(c)
+    requires ComposedValid(c, e1, e2)
+    requires knowns.Keys == ComposeEquivInputs(c, e1, e2)
+    requires forall np :: np in path ==> np.n in e1.sc
+    requires forall np :: np in prepath ==> np.n in e2.sc
+    requires EvaluateINPInnerRequirements(c, path, knowns)
+    requires EvaluateINPInnerRequirements(c, prepath + path, knowns)
+    ensures
+      var knowns_1 := ExtractMap(knowns, e1.inputs);
+      var knowns_2 := CalculateE2Inputs(c, e1, e2, knowns);
+      var np := Seq.Last(path);
+      (EvaluateINPInner(c, path, knowns) == EvaluateINPInner(c, path, knowns_1)) &&
+      (Simpl(EvaluateINPInner(c, path, knowns)) == Simpl(EvaluateINPInner(c, prepath+path, knowns)))
+    decreases |NodesNotInPath(c, prepath + path)|, 2
+  {
+    reveal ComposedValid();
+    reveal EquivValid();
+    var knowns_1 := ExtractMap(knowns, e1.inputs);
+    var knowns_2 := CalculateE2Inputs(c, e1, e2, knowns);
+    var np := Seq.Last(path);
+    var tail := Seq.DropLast(path);
+    assert Seq.HasNoDuplicates(path);
+    HasNoDuplicatesMeansHeadNotInTail(path);
+    assert np !in tail;
+    if np in e1.inputs {
+      assert EvaluateINPInner(c, path, knowns) == EvaluateINPInner(c, path, knowns_1);
+      assert Simpl(EvaluateINPInner(c, path, knowns)) == Simpl(EvaluateINPInner(c, prepath+path, knowns));
+    } else {
+      if np in c.PortSource {
+        var onp := c.PortSource[np];
+        assert onp.n in e1.sc;
+        if onp in path {
+          assert EvaluateINPInner(c, path, knowns) == EvaluateINPInner(c, path, knowns_1);
+          assert Simpl(EvaluateINPInner(c, path, knowns)) == Simpl(EvaluateINPInner(c, prepath+path, knowns));
+        } else {
+          NodesNotInPathDecreases(c, prepath+path, onp);
+          StillHasNoDuplicates(path, onp);
+          StillHasNoDuplicates(prepath + path, onp);
+          assert (prepath + path) + [onp] == prepath + (path + [onp]);
+          assert Seq.HasNoDuplicates(prepath + (path + [onp]));
+          EvaluateONPInnerComposed1(c, e1, e2, prepath, path + [onp], knowns);
+          assert EvaluateINPInner(c, path, knowns) == EvaluateINPInner(c, path, knowns_1);
+          assert Simpl(EvaluateINPInner(c, path, knowns)) == Simpl(EvaluateINPInner(c, prepath+path, knowns));
+        }
+      } else {
+        assert EvaluateINPInner(c, path, knowns) == EvaluateINPInner(c, path, knowns_1);
+        assert Simpl(EvaluateINPInner(c, path, knowns)) == Simpl(EvaluateINPInner(c, prepath+path, knowns));
+      }
+    }
+  }
+
+  lemma {:vcs_split_on_every_assert} EvaluateINPInnerComposed2(c: Circuit, e1: Equiv, e2: Equiv, path: seq<NP>, knowns: map<NP, bool>)
+    requires CircuitValid(c)
+    requires ComposedValid(c, e1, e2)
+    requires knowns.Keys == ComposeEquivInputs(c, e1, e2)
+    requires forall np :: np in path ==> np.n in e2.sc
+    requires EvaluateINPInnerRequirements(c, path, knowns)
+    ensures
+      var knowns_1 := ExtractMap(knowns, e1.inputs);
+      var knowns_2 := CalculateE2Inputs(c, e1, e2, knowns);
+      var np := Seq.Last(path);
+      (EvaluateINPInner(c, path, knowns) == EvaluateINPInner(c, path, knowns_2))
+    decreases |NodesNotInPath(c, path)|, 2
+  {
+    reveal ComposedValid();
+    reveal EquivValid();
+    var knowns_1 := ExtractMap(knowns, e1.inputs);
+    var knowns_2 := CalculateE2Inputs(c, e1, e2, knowns);
+    var np := Seq.Last(path);
+    var tail := Seq.DropLast(path);
+    assert Seq.HasNoDuplicates(path);
+    HasNoDuplicatesMeansHeadNotInTail(path);
+    assert np !in tail;
+    if np in e2.inputs {
+      if np in knowns {
+        assert EvaluateINPInner(c, path, knowns) == EvaluateINPInner(c, path, knowns_2);
+      } else {
+        var onp := c.PortSource[np];
+        assert onp.n in e1.sc;
+        assert onp !in path;
+        NodesNotInPathDecreases(c, path, onp);
+        StillHasNoDuplicates(path, onp);
+        LengthOneNoDuplicates([onp]);
+        EvaluateONPInnerComposed1(c, e1, e2, path, [onp], knowns);
+        assert (EvaluateONPInner(c, [onp], knowns) == EvaluateONPInner(c, [onp], knowns_1)); //  (1)
+        assert (EvaluateONPInner(c, path + [onp], knowns) == EvaluateONPInner(c, [onp], knowns)); // (2)
+        assert EvaluateINPInner(c, path, knowns) == EvaluateONPInner(c, path + [onp], knowns); // (3)
+        assert knowns_2[np] == e1.f(knowns_1)[onp]; // (4)
+        assert EvaluateONPInner(c, [onp], knowns_1) == EvalOk(e1.f(knowns_1)[onp]); // (5)
+
+        assert EvaluateINPInner(c, path, knowns_2) == EvalOk(knowns_2[np]); // by it's own def
+        assert EvaluateINPInner(c, path, knowns_2) == EvaluateONPInner(c, [onp], knowns_1); // by (4) and (5)
+        assert EvaluateINPInner(c, path, knowns_2) == EvaluateONPInner(c, [onp], knowns); // by (1)
+        assert EvaluateINPInner(c, path, knowns_2) == EvaluateONPInner(c, path + [onp], knowns); // by (2)
+        assert EvaluateINPInner(c, path, knowns_2) == EvaluateINPInner(c, path, knowns); // by (3)
+      }
+    } else {
+      if np in c.PortSource {
+        var onp := c.PortSource[np];
+        assert onp.n in e2.sc;
+        if onp in path {
+          assert EvaluateINPInner(c, path, knowns) == EvaluateINPInner(c, path, knowns_2);
+        } else {
+          NodesNotInPathDecreases(c, path, onp);
+          StillHasNoDuplicates(path, onp);
+          EvaluateONPInnerComposed2(c, e1, e2, path + [onp], knowns);
+          assert EvaluateINPInner(c, path, knowns) == EvaluateINPInner(c, path, knowns_2);
+        }
+      } else {
+        assert EvaluateINPInner(c, path, knowns) == EvaluateINPInner(c, path, knowns_2);
+      }
+    }
+  }
+
+  lemma {:vcs_split_on_every_assert} EvaluateONPInnerComposed1(c: Circuit, e1: Equiv, e2: Equiv, prepath: seq<NP>, path: seq<NP>, knowns: map<NP, bool>)
+    requires CircuitValid(c)
+    requires ComposedValid(c, e1, e2)
+    requires knowns.Keys == ComposeEquivInputs(c, e1, e2)
+    requires EvaluateONPInnerRequirements(c, prepath + path, knowns)
+    requires EvaluateONPInnerRequirements(c, path, knowns)
+    requires forall np :: np in path ==> np.n in e1.sc
+    requires forall np :: np in prepath ==> np.n in e2.sc
+    ensures
+      var knowns_1 := ExtractMap(knowns, e1.inputs);
+      (EvaluateONPInner(c, path, knowns) == EvaluateONPInner(c, path, knowns_1)) &&
+      (Simpl(EvaluateONPInner(c, prepath + path, knowns)) == Simpl(EvaluateONPInner(c, path, knowns)))
+    decreases |NodesNotInPath(c, prepath + path)|, 4
+  {
+    reveal ComposedValid();
+    reveal EquivValid();
+    var knowns_1 := ExtractMap(knowns, e1.inputs);
+    var np := Seq.Last(path);
+    Seq.LemmaAppendLast(prepath, path);
+    assert np == Seq.Last(prepath + path);
+    if np in knowns {
+      assert np in knowns_1;
+      assert EvaluateONPInner(c, path, knowns) == EvaluateONPInner(c, path, knowns_1);
+      assert Simpl(EvaluateONPInner(c, prepath + path, knowns)) == Simpl(EvaluateONPInner(c, path, knowns));
+    } else {
+      var nk := c.NodeKind[np.n];
+      match nk
+        case CXor() => {
+          EvaluateONPBinaryComposed1(c, e1, e2, prepath, path, knowns);
+        }
+        case CAnd() => {
+          EvaluateONPBinaryComposed1(c, e1, e2, prepath, path, knowns);
+        }
+        case CInv() => {
+          EvaluateONPUnaryComposed1(c, e1, e2, prepath, path, knowns);
+        }
+        case CConst(b) => {}
+        case CInput() => {}
+        case CSeq() => {}
+      assert EvaluateONPInner(c, path, knowns) == EvaluateONPInner(c, path, knowns_1);
+      assert Simpl(EvaluateONPInner(c, prepath + path, knowns)) == Simpl(EvaluateONPInner(c, path, knowns));
+    }
+    assert EvaluateONPInner(c, path, knowns) == EvaluateONPInner(c, path, knowns_1);
+    assert Simpl(EvaluateONPInner(c, prepath + path, knowns)) == Simpl(EvaluateONPInner(c, path, knowns));
+  }
+
+  lemma {:vcs_split_on_every_assert} EvaluateONPInnerComposed2(c: Circuit, e1: Equiv, e2: Equiv, path: seq<NP>, knowns: map<NP, bool>)
+    requires CircuitValid(c)
+    requires ComposedValid(c, e1, e2)
+    requires knowns.Keys == ComposeEquivInputs(c, e1, e2)
+    requires EvaluateONPInnerRequirements(c, path, knowns)
+    requires forall np :: np in path ==> np.n in e2.sc
+    ensures
+      var knowns_2 := CalculateE2Inputs(c, e1, e2, knowns);
+      var np := path[|path|-1];
+      (EvaluateONPInner(c, path, knowns) == EvaluateONPInner(c, path, knowns_2))
+    decreases |NodesNotInPath(c, path)|, 4
+  {
+    reveal ComposedValid();
+    reveal EquivValid();
+    var knowns_2 := CalculateE2Inputs(c, e1, e2, knowns);
+    var np := Seq.Last(path);
+    if np in knowns {
+      assert np in knowns_2;
+      assert EvaluateONPInner(c, path, knowns) == EvaluateONPInner(c, path, knowns_2);
+    } else {
+      var nk := c.NodeKind[np.n];
+      match nk
+        case CXor() => {
+          EvaluateONPBinaryComposed2(c, e1, e2, path, knowns);
+        }
+        case CAnd() => {
+          EvaluateONPBinaryComposed2(c, e1, e2, path, knowns);
+        }
+        case CInv() => {
+          EvaluateONPUnaryComposed2(c, e1, e2, path, knowns);
+        }
+        case CConst(b) => {}
+        case CInput() => {}
+        case CSeq() => {}
+    }
+  }
+
+  lemma {:vcs_split_on_every_assert} EvaluateComposedInner(c: Circuit, e1: Equiv, e2: Equiv, np: NP, knowns: map<NP, bool>)
+    requires CircuitValid(c)
+    requires ComposedValid(c, e1, e2)
+    requires knowns.Keys == ComposeEquivInputs(c, e1, e2)
+    requires ONPValid(c, np) || INPValid(c, np)
+    requires np.n in (e1.sc + e2.sc)
+    requires np in e1.outputs || np in e2.outputs
+    ensures
+      var knowns_1 := ExtractMap(knowns, e1.inputs);
+      var knowns_2 := CalculateE2Inputs(c, e1, e2, knowns);
+      (np.n in e1.sc ==> Evaluate(c, np, knowns_1) == Evaluate(c, np, knowns)) &&
+      (np.n in e2.sc ==> Evaluate(c, np, knowns_2) == Evaluate(c, np, knowns))
+  {
+    var prepath: seq<NP> := [];
+    var path := [np];
+    assert np == path[|path|-1];
+    assert PathValid(c, path);
+
+    var knowns_1 := ExtractMap(knowns, e1.inputs);
+    var knowns_2 := CalculateE2Inputs(c, e1, e2, knowns);
+
+    LengthOneNoDuplicates(path);
+    LengthOneNoDuplicates(prepath + path);
+    if ONPValid(c, np) {
+      if np.n in e1.sc {
+        EvaluateONPInnerComposed1(c, e1, e2, prepath, path, knowns);
+        assert EvaluateONPInner(c, path, knowns) == EvaluateONPInner(c, path, knowns_1);
+      } else {
+        EvaluateONPInnerComposed2(c, e1, e2, path, knowns);
+        assert EvaluateONPInner(c, path, knowns) == EvaluateONPInner(c, path, knowns_2);
+      }
+    } else {
+      if np.n in e1.sc {
+        EvaluateINPInnerComposed1(c, e1, e2, prepath, path, knowns);
+        assert EvaluateINPInner(c, path, knowns) == EvaluateINPInner(c, path, knowns_1);
+      } else {
+        EvaluateINPInnerComposed2(c, e1, e2, path, knowns);
+        assert EvaluateINPInner(c, path, knowns) == EvaluateINPInner(c, path, knowns_2);
+      }
+    }
+    reveal ComposedValid();
+    if np.n in e1.sc {
+      assert np.n !in e2.sc;
+      assert Evaluate(c, np, knowns) == Evaluate(c, np, knowns_1);
+    } else {
+      assert np.n in e2.sc;
+      assert Evaluate(c, np, knowns) == Evaluate(c, np, knowns_2);
+    }
+  }
+
+  lemma {:vcs_split_on_every_assert} EvaluateComposed(c: Circuit, e1: Equiv, e2: Equiv, np: NP, knowns: map<NP, bool>)
+    requires CircuitValid(c)
+    requires ComposedValid(c, e1, e2)
+    requires knowns.Keys == ComposeEquivInputs(c, e1, e2)
+    requires ONPValid(c, np) || INPValid(c, np)
+    requires np.n in (e1.sc + e2.sc)
+    requires np in e1.outputs || np in e2.outputs
+    ensures
+      var e := ComposeEquiv(c, e1, e2);
+      e.f.requires(knowns) &&
+      np in e.f(knowns) &&
+      Evaluate(c, np, knowns) == EvalOk(e.f(knowns)[np])
+  {
+    EvaluateComposedInner(c, e1, e2, np, knowns);
+    var e := ComposeEquiv(c, e1, e2);
+    assert EquivValid(c, e);
+    {
+      reveal EquivValid();
+      assert e.f.requires(knowns);
+      assert np in e.f(knowns);
+    }
+
+    var knowns_1 := ExtractMap(knowns, e1.inputs);
+    var knowns_2 := CalculateE2Inputs(c, e1, e2, knowns);
+
+
+    //assert forall np :: np in e1.inputs + e1.outputs ==> np.n in e1.sc;
+    //assert forall np :: np in e2.inputs + e2.outputs ==> np.n in e2.sc;
+    //assert SetsNoIntersection(e1.inputs+e1.outputs, e2.inputs+e2.outputs);
+
+    //var mf1 := EtoMf(e1);
+    //var mf2 := EtoMf(e2);
+    //EValidMfValid(c, e1);
+    //EValidMfValid(c, e2);
+    //var e2_inputs_from_e1_keys := NPBetweenSubcircuits(c, e2.sc, e1.sc);
+    //var e2_inputs_from_e1 := (map np | np in e2_inputs_from_e1_keys :: np := c.PortSource[np]);
+    //assert e.f(knowns) == ComposeMapFunction(mf1, mf2, e2_inputs_from_e1, knowns);
+
+    if np in e1.outputs {
+      {
+        reveal ComposedValid();
+        reveal EquivValid();
+        assert Evaluate(c, np, knowns_1) == EvalOk(e1.f(knowns_1)[np]);
+      }
+      assert Evaluate(c, np, knowns) == Evaluate(c, np, knowns_1);
+      assert EvalOk(e1.f(knowns_1)[np]) == EvalOk(e.f(knowns)[np]);
+      assert Evaluate(c, np, knowns) == EvalOk(e.f(knowns)[np]);
+    } else {
+      assert np in e2.outputs;
+      {
+        reveal ComposedValid();
+        reveal EquivValid();
+        assert Evaluate(c, np, knowns_2) == EvalOk(e2.f(knowns_2)[np]);
+      }
+      assert Evaluate(c, np, knowns) == Evaluate(c, np, knowns_2);
+      assert EvalOk(e2.f(knowns_2)[np]) == EvalOk(e.f(knowns)[np]);
+      assert Evaluate(c, np, knowns) == EvalOk(e.f(knowns)[np]);
+
+    }
+  }
+
+  lemma {:vcs_split_on_every_assert} ComposeEquivCorrect(c: Circuit, e1: Equiv, e2: Equiv)
+    requires ComposedValid(c, e1, e2)
+    ensures
+      var r := ComposeEquiv(c, e1, e2);
+      CircuitValid(c) &&
+      EquivValid(c, r) &&
+      EquivTrue(c, r)
+  {
+    reveal ComposedValid();
+    reveal EquivValid();
+    var combined_input_keys := ComposeEquivInputs(c, e1, e2);
+    var e := ComposeEquiv(c, e1, e2);
+    assert EquivValid(c, e);
+    forall knowns: map<NP, bool> | (knowns.Keys == e.inputs)
+      ensures
+        e.f.requires(knowns) &&
+        (forall np :: np in e.outputs ==>
+          np in e.f(knowns) &&
+          (Evaluate(c, np, knowns) == EvalOk(e.f(knowns)[np])))
+    {
+      forall np | np in e.outputs
+        ensures
+          e.f.requires(knowns) &&
+          np in e.f(knowns) &&
+          (Evaluate(c, np, knowns) == EvalOk(e.f(knowns)[np]))
+      {
+        EvaluateComposed(c, e1, e2, np, knowns);
+      }
+    }
+    assert EquivTrue(c, e);
+  }
+
+}
