Attempt2/ConservedSubcircuit.dfy
@@ -1,0 +1,201 @@
+module ConservedSubcircuit {
+
+  import opened Circ
+  import opened Eval
+
+  // To show that the rest of the graph is unchanged I need to show that
+  // there is a set of nodes which have the same n.
+  // There are no connections from those nodes to anything new without getting blocked by a known.
+  // The result of an Evaluate should be the same.
+
+  // We define a subgraph as all the nodes in the subgraph together with all the INPs that form the
+  // upper boundary (not really necessary, can probably simplify in the future)
+  datatype Subcircuit = Subcircuit(
+    nodes: set<CNode>,
+    boundary: set<NP>
+  )
+
+  predicate SubcircuitValid(c: Circuit, sc: Subcircuit)
+  {
+    (forall np :: np in sc.boundary ==> INPValid(c, np) || ONPValid(c, np)) &&
+    (forall n :: n in sc.nodes ==> n in c.NodeKind) &&
+    (forall np :: np in sc.boundary ==> np.n in sc.nodes) &&
+    (forall np: NP :: np.n in sc.nodes && np in c.PortSource && np !in sc.boundary ==>
+      c.PortSource[np].n in sc.nodes)
+  }
+
+  ghost predicate SubcircuitConserved(ca: Circuit, cb: Circuit, sc: set<CNode>)
+  {
+    (forall n :: n in sc ==> n in  ca.NodeKind && n in cb.NodeKind) &&
+    (forall n :: n in sc ==> ca.NodeKind[n] == cb.NodeKind[n]) &&
+    (forall n :: n in sc ==> ca.NodeKind[n] == cb.NodeKind[n]) &&
+    (forall np: NP :: (np in ScInputBoundary(ca, sc)) == (np in ScInputBoundary(cb, sc))) &&
+    (forall np: NP :: (np !in ScInputBoundary(ca, sc)) && np.n in sc ==> (np in ca.PortSource) == (np in cb.PortSource)) &&
+    (forall np: NP :: (np !in ScInputBoundary(ca, sc)) && np.n in sc && np in ca.PortSource ==> ca.PortSource[np] == cb.PortSource[np])
+  }
+
+  ghost predicate ConservedValid(ca: Circuit, cb: Circuit, e: Equiv, known: map<NP, bool>)
+  {
+    CircuitValid(ca) && CircuitValid(cb) &&
+    EquivValid(ca, e) && EquivValid(cb, e) &&
+    SubcircuitConserved(ca, cb, e.sc) &&
+    (forall np :: np in e.inputs ==> np in known) &&
+    (forall np :: np in known ==> np.n in e.sc)
+  }
+
+  lemma EvaluateINPInnerConserved(
+    ca: Circuit, cb: Circuit, e: Equiv, path: seq<NP>, knowns: map<NP, bool>)
+    requires ConservedValid(ca, cb, e, knowns)
+    requires |path| > 0
+    requires forall np :: np in path ==> np.n in e.sc
+    requires PathValid(ca, path)
+    requires Seq.HasNoDuplicates(path)
+    requires INPValid(ca, path[|path|-1])
+    ensures PathValid(cb, path)
+    ensures
+      EvaluateINPInner(ca, path, knowns) == EvaluateINPInner(cb, path, knowns)
+    decreases |NodesNotInPath(ca, path)|, 2
+  {
+    reveal EquivValid();
+    var head := path[|path|-1];
+    var tail := path[..|path|-1];
+    if head in knowns {
+    } else {
+      if head in ca.PortSource {
+        var onp := ca.PortSource[head];
+        if onp in path {
+        } else {
+          NodesNotInPathDecreases(ca, path, onp);
+          StillHasNoDuplicates(path, onp);
+          EvaluateONPInnerConserved(ca, cb, e, path + [onp], knowns);
+        }
+      } else {
+      }
+    }
+  }
+
+  lemma EvaluateONPBinaryConserved(
+      ca: Circuit, cb: Circuit, e: Equiv, path: seq<NP>, knowns: map<NP, bool>)
+    requires ConservedValid(ca, cb, e, knowns)
+    requires |path| > 0
+    requires ONPValid(ca, path[|path|-1])
+    requires path[|path|-1] !in knowns
+    requires forall np :: np in path ==> np.n in e.sc
+    requires
+      var nk := ca.NodeKind[path[|path|-1].n];
+      nk.CXor? || nk.CAnd?
+    requires PathValid(ca, path)
+    requires Seq.HasNoDuplicates(path)
+    ensures PathValid(cb, path)
+    ensures EvaluateONPBinary(ca, path, knowns) == EvaluateONPBinary(cb, path, knowns)
+    decreases |NodesNotInPath(ca, path)|, 3
+  {
+    reveal EquivValid();
+    var nk := ca.NodeKind[path[|path|-1].n];
+    var head := path[|path|-1];
+    assert NodeValid(ca, head.n);
+    var inp_0 := NP(head.n, INPUT_0);
+    var inp_1 := NP(head.n, INPUT_1);
+    if inp_0 in path {
+    } else if inp_1 in path {
+    } else {
+      NodesNotInPathDecreases(ca, path, inp_0);
+      NodesNotInPathDecreases(ca, path, inp_1);
+      StillHasNoDuplicates(path, inp_0);
+      StillHasNoDuplicates(path, inp_1);
+      EvaluateINPInnerConserved(ca, cb, e, path + [inp_0], knowns);
+      EvaluateINPInnerConserved(ca, cb, e, path + [inp_1], knowns);
+    }
+  }
+
+  lemma EvaluateONPUnaryConserved(
+      ca: Circuit, cb: Circuit, e: Equiv, path: seq<NP>, knowns: map<NP, bool>)
+    requires ConservedValid(ca, cb, e, knowns)
+    requires |path| > 0
+    requires ONPValid(ca, path[|path|-1])
+    requires path[|path|-1] !in knowns
+    requires ca.NodeKind[path[|path|-1].n].CInv?
+    requires PathValid(ca, path)
+    requires forall np :: np in path ==> np.n in e.sc
+    requires Seq.HasNoDuplicates(path)
+    ensures PathValid(cb, path)
+    ensures EvaluateONPUnary(ca, path, knowns) == EvaluateONPUnary(cb, path, knowns)
+    decreases |NodesNotInPath(ca, path)|, 3
+  {
+    reveal EquivValid();
+    var head := path[|path|-1];
+    var inp_0 := NP(head.n, INPUT_0);
+    if inp_0 in path {
+    } else {
+      NodesNotInPathDecreases(ca, path, inp_0);
+      StillHasNoDuplicates(path, inp_0);
+      EvaluateINPInnerConserved(ca, cb, e, path + [inp_0], knowns);
+    }
+  }
+
+  lemma EvaluateONPInnerConserved(
+      ca: Circuit, cb: Circuit, e: Equiv, path: seq<NP>, knowns: map<NP, bool>)
+    requires ConservedValid(ca, cb, e, knowns)
+    requires EvaluateONPInnerRequirements(ca, path, knowns)
+    requires forall np :: np in path ==> np.n in e.sc
+    ensures PathValid(cb, path)
+    ensures EvaluateONPInner(ca, path, knowns) == EvaluateONPInner(cb, path, knowns)
+    decreases |NodesNotInPath(ca, path)|, 4
+  {
+    reveal EquivValid();
+    var head := path[|path|-1];
+    if head in knowns {
+    } else {
+      var nk := ca.NodeKind[head.n];
+      match nk
+        case CXor() => EvaluateONPBinaryConserved(ca, cb, e, path, knowns);
+        case CAnd() => EvaluateONPBinaryConserved(ca, cb, e, path, knowns);
+        case CInv() => EvaluateONPUnaryConserved(ca, cb, e, path, knowns);
+        case CConst(b) => {}
+        case CInput() => {}
+        case CSeq() => {}
+    }
+  }
+
+  lemma EvaluateConserved(ca: Circuit, cb: Circuit, e: Equiv, o: NP, known: map<NP, bool>)
+    requires ConservedValid(ca, cb, e, known)
+    requires o.n in e.sc
+    requires INPValid(ca, o) || ONPValid(ca, o)
+    ensures INPValid(cb, o) || ONPValid(cb, o)
+    ensures Evaluate(ca, o, known) == Evaluate(cb, o, known)
+  {
+    reveal EquivValid();
+    assert PathValid(ca, [o]);
+    LengthOneNoDuplicates([o]);
+    if INPValid(ca, o) {
+      EvaluateINPInnerConserved(ca, cb, e, [o], known);
+    } else {
+      EvaluateONPInnerConserved(ca, cb, e, [o], known);
+    }
+  }
+
+  lemma EquivConserved(ca: Circuit, cb: Circuit, e: Equiv)
+    requires CircuitValid(ca)
+    requires CircuitValid(cb)
+    requires SubcircuitConserved(ca, cb, e.sc)
+    requires forall np :: np in ScOutputBoundary(ca, e.sc) ==> np in e.outputs
+    requires forall np :: np in ScOutputBoundary(cb, e.sc) ==> np in e.outputs
+    ensures EquivValid(ca, e) == EquivValid(cb, e)
+    ensures EquivValid(ca, e) ==> EquivTrue(ca, e) == EquivTrue(cb, e)
+  {
+    reveal EquivValid();
+    assert EquivValid(ca, e) == EquivValid(cb, e);
+    if EquivValid(ca, e) {
+      forall knowns: map<NP, bool> | knowns.Keys == e.inputs
+        ensures forall np :: np in e.outputs ==> Evaluate(ca, np, knowns) == Evaluate(cb, np, knowns)
+      {
+        forall np | np in e.outputs
+          ensures Evaluate(ca, np, knowns) == Evaluate(cb, np, knowns)
+        {
+          EvaluateConserved(ca, cb, e, np, knowns);
+          assert Evaluate(ca, np, knowns) == Evaluate(cb, np, knowns);
+        }
+      }
+    }
+  }
+}
