Attempt2/MapFunction.dfy
@@ -1,0 +1,64 @@
+module MapFunction {
+
+  import opened Circ
+  import opened Utils
+  //import opened Compose
+  //import opened Eval
+
+  datatype MapFunction = MapFunction(
+    inputs: set<NP>,
+    outputs: set<NP>,
+    f: map<NP, bool> --> map<NP, bool>
+  )
+
+  ghost predicate MapFunctionValid(mf: MapFunction)
+  {
+    (forall x: map<NP, bool> :: x.Keys == mf.inputs ==> mf.f.requires(x)) &&
+    (forall x: map<NP, bool> :: x.Keys == mf.inputs ==> mf.f(x).Keys == mf.outputs) &&
+    SetsNoIntersection(mf.inputs, mf.outputs)
+  }
+
+  function GetInputs2(
+      mf1: MapFunction, mf2: MapFunction, connection: map<NP, NP>, knowns: map<NP, bool>): map<NP, bool>
+    requires MapFunctionValid(mf1)
+    requires MapFunctionValid(mf2)
+    requires forall np :: np in connection.Keys ==> np in mf2.inputs
+    requires forall np :: np in connection.Values ==> np in mf1.outputs
+    requires SetsNoIntersection(mf1.inputs + mf1.outputs, mf2.inputs + mf2.outputs)
+    requires
+        var b: set<NP> := (mf1.inputs + mf2.inputs - connection.Keys);
+        knowns.Keys == b
+  {
+    var inputs := mf1.inputs + mf2.inputs - connection.Keys;
+    var outputs := mf1.outputs + mf2.outputs;
+    var inputs_1 := ExtractMap(knowns, mf1.inputs);
+    var outputs_1 := mf1.f(inputs_1);
+    assert outputs_1.Keys == mf1.outputs;
+    var connected := (map np | np in connection :: np := outputs_1[connection[np]]);
+    assert connected.Keys == connection.Keys;
+    var combined_map := AddMaps(knowns, connected);
+    assert combined_map.Keys == mf1.inputs + mf2.inputs;
+    var inputs_2 := ExtractMap(combined_map, mf2.inputs);
+    inputs_2
+  }
+
+  function {:vcs_split_on_every_assert} ComposeMapFunction(
+      mf1: MapFunction, mf2: MapFunction, connection: map<NP, NP>, knowns: map<NP, bool>): map<NP, bool>
+    requires MapFunctionValid(mf1)
+    requires MapFunctionValid(mf2)
+    requires forall np :: np in connection.Keys ==> np in mf2.inputs
+    requires forall np :: np in connection.Values ==> np in mf1.outputs
+    requires SetsNoIntersection(mf1.inputs + mf1.outputs, mf2.inputs + mf2.outputs)
+    requires
+        var b: set<NP> := (mf1.inputs + mf2.inputs - connection.Keys);
+        knowns.Keys == b
+  {
+    var inputs_1 := ExtractMap(knowns, mf1.inputs);
+    var outputs_1 := mf1.f(inputs_1);
+    var inputs_2 := GetInputs2(mf1, mf2, connection, knowns);
+    var outputs_2 := mf2.f(inputs_2);
+    var combined_outputs := AddMaps(outputs_1, outputs_2);
+    combined_outputs
+  }
+
+}
