Attempt2/Utils.dfy
@@ -1,0 +1,39 @@
+module Utils {
+
+  predicate SetsNoIntersection<T>(a: set<T>, b: set<T>)
+  {
+    forall x :: !(x in a && x in b)
+  }
+    
+  function ExtractMap<T, U>(a: map<T, U>, k: set<T>): (r: map<T, U>)
+    requires forall x :: x in k ==> x in a
+    ensures r.Keys == k
+    ensures forall x :: x in k ==> r[x] == a[x]
+  {
+    (map x | x in k :: a[x])
+  }
+
+  function CombineSets<T>(sc1: set<T>, sc2: set<T>): (r: set<T>)
+    requires SetsNoIntersection(sc1, sc2)
+  {
+    sc1 + sc2
+  }
+
+  function AddMaps<T, U>(a: map<T, U>, b: map<T, U>): (r: map<T, U>)
+    requires SetsNoIntersection(a.Keys, b.Keys)
+    ensures r.Keys == a.Keys + b.Keys
+    ensures forall x :: x in a ==> r[x] == a[x]
+    ensures forall x :: x in b ==> r[x] == b[x]
+    decreases |b|
+  {
+    if |b| == 0 then
+      a
+    else
+      var x :| x in b;
+      var new_a := a[x := b[x]];
+      var new_b := b - {x};
+      AddMaps(new_a, new_b)
+  }
+
+
+}
